\documentclass[12pt]{report}
\usepackage{epsfig,amssymb,amsmath,amsfonts,esdiff}
\begin{document}
\date{\today}
This is one of the tasks I had to do from last weeks meeting. Show that
\begin{eqnarray*} 
    \ddot{x} &=& -\frac{1}{r^2}\left(gx^2 + yv^2\right)\\
    \ddot{y} &=& -\frac{1}{r^2}\left(gx^2 + v^2y\right)
\end{eqnarray*} 
Given
\begin{eqnarray}
    x^2 + y^2 &=& r^2\\
    \ddot{x} &=& \frac{2\lambda x}{m}\\
    \ddot{y} &=& \frac{-mg + 2\lambda y}{m}\\
    x\ddot{x} + \dot{x}^2 + y\ddot{y} + \dot{y}^2 &=& 0
\end{eqnarray}
Substituting 2 and 3 in 4
\begin{eqnarray*}
    x\frac{2\lambda x}{m} + \dot{x}^2 + y\frac{-mg + 2\lambda y}{m} + \dot{y}^2
    &=& 0\\
    \frac{2\lambda}{m}(x^2 + y^2) + \dot{x}^2 - gy + \dot{y}^2 &=& 0\\
    \frac{2\lambda}{m}r^2 + v^2 - gy = 0\\
    \lambda = \frac{m(gy - v^2)}{2r^2}
\end{eqnarray*}
Substituting into 3
\begin{eqnarray*}
    \ddot{y} &=& \frac{-mg + 2\frac{m(gy - v^2)}{2r^2} y}{m}\\
    \ddot{y} &=& -g + \frac{y\left(gy - v^2\right)}{r^2}\\
    \ddot{y} &=& -g + \frac{g\left(r^2 - x^2\right) - v^2y}{r^2}\\
    \ddot{y} &=& -\frac{1}{r^2}\left(gx^2 + v^2y\right)
\end{eqnarray*}
Similarly sustituting $\lambda$ into 2 and solving for $\ddot{x}$
\begin{eqnarray*}
    \ddot{x} &=& -\frac{1}{r^2}\left(gx^2 + yv^2\right)
\end{eqnarray*}
\end{document}

